DataflowSyntax.v
@@ -4,7 +4,7 @@ Require Import Rustre.Common.
 (** * Dataflow language *)
 
 Inductive clock : Set :=
-| Cbase : clock                           (* base clock *)
+| Cbase : clock                          (* base clock *)
 | Con : clock -> ident -> bool -> clock. (* subclock *)
 
 Record var_dec : Set := mk_var { v_name : ident;
@@ -13,7 +13,7 @@ Record var_dec : Set := mk_var { v_name : ident;
 (** ** Syntax *)
 
 (* TODO: laexp: would be nicer if it were a record *)
-Inductive laexp : Set :=
+Inductive laexp : Type :=
   | LAexp : clock -> lexp -> laexp
 with lexp : Type :=
   | Econst : const -> lexp
@@ -33,14 +33,31 @@ with cexp : Type :=
 Inductive equation : Type :=
   | EqDef : ident -> caexp -> equation
   | EqApp : ident -> ident -> laexp -> equation
-(*  | EqFby : ident -> const -> caexp -> equation*). (* Lionel added this one *)
+  | EqFby : ident -> const -> laexp -> equation.
 
 Record node : Type := mk_node {
   n_name : ident;
   n_input : var_dec;
   n_output : var_dec;
   n_eqs : list equation
-}.
+                        }.
+
+(** ** Predicates *)
+
+Require Coq.MSets.MSets.
+
+Module PS := Coq.MSets.MSetPositive.PositiveSet.
+
+Fixpoint freevar_lexp' (e : lexp) (fvs : PS.t) : PS.t :=
+  match e with
+    | Econst c => fvs
+    | Evar x => PS.add x fvs
+    | Ewhen ae c x => freevar_laexp' ae fvs
+  end
+with freevar_laexp' (lae : laexp) (fvs : PS.t) : PS.t :=
+  match lae with
+    | LAexp ck e => freevar_lexp' e fvs
+  end.
 
 (** The map containing global definitions. *)
 Require Coq.FSets.FMapPositive.
