SynchronousNat.v
@@ -1,0 +1,116 @@
+Require Import Coq.FSets.FMapPositive.
+Require Import Rustre.Common.
+Require Import Rustre.DataflowSyntax.
+
+Inductive value :=
+  | absent
+  | present (v : const).
+Coercion present : const >-> value.
+
+Module PM := PositiveMap.
+
+Definition stream := nat -> value.
+Definition cstream := nat -> bool.
+
+(** Synchronous functions *)
+
+(* With auxiliary hold function. *)
+
+Inductive holdR (v0: const) (xs: stream) : nat -> value -> Prop :=
+| holdR0:
+    holdR v0 xs 0 v0
+| holdR_absent:
+    forall v n,
+      xs n = absent ->
+      holdR v0 xs n v ->
+      holdR v0 xs (S n) v
+| holdR_present:
+    forall n,
+      xs n <> absent ->
+      holdR v0 xs (S n) (xs n).
+
+Inductive fbyR (v0: const) (xs: stream) : nat -> value -> Prop :=
+| fbyR_absent:
+    forall n,
+      xs n = absent ->
+      fbyR v0 xs n absent
+| fbyR_present:
+    forall v n,
+      xs n <> absent ->
+      holdR v0 xs n v ->
+      fbyR v0 xs n v.
+
+Fixpoint hold (v0: const) (xs: stream) (n: nat) : value :=
+  match n with
+  | 0 => v0
+  | S m => match xs m with
+           | absent => hold v0 xs m
+           | hv => hv
+           end
+  end.
+
+Definition fby (v0: const) (xs: stream) (n: nat) : value :=
+  match xs n with
+  | absent => absent
+  | _ => hold v0 xs n
+  end.
+
+Lemma hold_rel1: forall v0 xs n, holdR v0 xs n (hold v0 xs n).
+Proof.
+  induction n.
+  - cbv; auto using holdR0.
+  - simpl. case_eq (xs n).
+    + auto using holdR_absent.
+    + intros v xsn; rewrite <- xsn.
+      apply holdR_present.
+      rewrite xsn; discriminate.
+Qed.
+
+Lemma hold_rel2: forall v0 xs n v, holdR v0 xs n v -> hold v0 xs n = v.
+Proof.
+  induction n as [|n IH].
+  - inversion 1; auto.
+  - intros v H; inversion_clear H as [|? ? xsn HR|? H1].
+    + simpl; rewrite xsn; apply (IH v HR).
+    + simpl. case_eq (xs n). contradiction. trivial.
+Qed.
+
+Lemma hold_rel: forall v0 xs n v, hold v0 xs n = v <-> holdR v0 xs n v.
+Proof.
+  split.
+  intro H; rewrite <- H; apply hold_rel1.
+  apply hold_rel2.
+Qed.
+    
+Lemma fby_rel1: forall v0 xs n, fbyR v0 xs n (fby v0 xs n).
+Proof.
+  intros v0 xs n.
+  unfold fby.
+  case_eq (xs n).
+  - auto using fbyR_absent.
+  - intros v xsn.
+    apply fbyR_present.
+    + rewrite xsn; discriminate.
+    + apply hold_rel; reflexivity.
+Qed.
+
+Lemma fby_rel2: forall v0 xs n v, fbyR v0 xs n v -> fby v0 xs n = v.
+Proof.
+  induction n.
+  - inversion_clear 1 as [ ? H0 | ? ? ? HR].
+    + unfold fby; rewrite H0; reflexivity.
+    + unfold fby; case_eq (xs 0).
+      contradiction. intros v1 xsn; apply hold_rel2; exact HR.
+  - inversion_clear 1 as [ ? H0 | ? ? ? HR].
+    + unfold fby; rewrite H0; reflexivity.
+    + unfold fby; case_eq (xs (S n)).
+      contradiction. intros v1 xsn; apply hold_rel2; exact HR.
+Qed.
+
+Lemma fby_rel: forall v0 xs n v, fby v0 xs n = v <-> fbyR v0 xs n v.
+Proof.
+  split.
+  intro H; rewrite <- H; apply fby_rel1.
+  apply fby_rel2.
+Qed.
+
