TranslationNatSemantics.v
@@ -5,6 +5,81 @@ Require Import Rustre.DataflowSyntax.
 Require Import Rustre.DataflowNatSemantics.
 Require Import Rustre.Translation.
 
+Module PM := PositiveMap.
+
+(*
+Lemma sem_laexp_some:
+  forall H ck ce n v,
+    sem_laexp H (LAexp ck ce) n (Some v) ->
+    sem_lexp H ce n (Some v).
+Proof.
+  intros until v.
+  inversion 1.
+  apply H5.
+Qed.
+*)
+
+Lemma compat_laexp:
+  forall (H: history)(menv: memoryEnv)(env: valueEnv),
+  forall (lae: laexp),
+  forall (n: nat)(v: const),
+    (forall x, PS.In x (freevar_laexp lae) ->
+               PM.find x (H n) = Some (PM.find x env)) ->
+    (sem_laexp H lae n (Some v)
+    <->
+    exp_eval menv env (translate_laexp lae) v).
+Proof.
+  intros until v.
+  elim lae.
+  intros k e.
+  elim e.
+  - intros c.
+    split.
+    + simpl.
+      intro H1.
+      inversion H1.
+      inversion H6.
+      constructor.
+    + simpl.
+      intro H1.
+      inversion H1.
+      constructor.
+      constructor.
+
+      sem_clock H k n true
+                
+      destruct H1.
+    
+    inversion 0.
+    Search (_ <-> _).
+    Check (iff_to_and).
+    Locate "<->".
+    Print iff.
+
+           HIN HH.
+  simpl.
+  inversion 0.
+Print econst.
+  
+  Check (econst).
+  Check (SLtick).
+  apply econst.
+  case v.
+  discriminate.
+  
+  intros HIN HH.
+
+  intros c e.
+  elim e.
+  simpl.
+
+
+  
+
+
+
+
+
 
 (* * Compatibility & equivalences *)
 
